BPlusTree_Split.thy
@@ -13,14 +13,10 @@ text "Linear split is similar to well known functions, therefore a quick proof c
 fun linear_split where "linear_split xs x = (takeWhile (\<lambda>(_,s). s<x) xs, dropWhile (\<lambda>(_,s). s<x) xs)"
 fun linear_split_list where "linear_split_list xs x = (takeWhile (\<lambda>s. s<x) xs, dropWhile (\<lambda>s. s<x) xs)"
 
-global_interpretation bplustree_linear_search: split_full linear_split linear_split_list
-  (* the below definitions are required to be set here for evaluating example code... *)
-  defines bplustree_ls_isin = bplustree_linear_search.isin 
-    and bplustree_ls_isin_list = bplustree_linear_search.isin_list 
-    and bplustree_ls_ins = bplustree_linear_search.ins
-    and bplustree_ls_insert = bplustree_linear_search.insert
-    and bplustree_ls_del = bplustree_linear_search.del
-    and bplustree_ls_delete = bplustree_linear_search.delete
+global_interpretation bplustree_linear_search_list: split_list linear_split_list
+  defines bplustree_ls_isin_list = bplustree_linear_search_list.isin_list 
+    and bplustree_ls_insert_list = bplustree_linear_search_list.insert_list
+    and bplustree_ls_delete_list = bplustree_linear_search_list.delete_list
   apply unfold_locales
   unfolding linear_split.simps
     apply (auto split: list.splits)
@@ -28,44 +24,61 @@ global_interpretation bplustree_linear_search: split_full linear_split linear_sp
     by (metis (no_types, lifting) case_prodD in_set_conv_decomp takeWhile_eq_all_conv takeWhile_idem)
   subgoal
     by (metis case_prod_conv hd_dropWhile le_less_linear list.sel(1) list.simps(3))
+  done
+
+global_interpretation bplustree_linear_search:
+    split_set linear_split bplustree_ls_isin_list bplustree_ls_insert_list bplustree_ls_delete_list
+  (* the below definitions are required to be set here for evaluating example code... *)
+  defines bplustree_ls_isin = bplustree_linear_search.isin 
+    and bplustree_ls_ins = bplustree_linear_search.ins
+    and bplustree_ls_insert = bplustree_linear_search.insert
+    and bplustree_ls_del = bplustree_linear_search.del
+    and bplustree_ls_delete = bplustree_linear_search.delete
+  apply unfold_locales
+  unfolding linear_split.simps
+  subgoal by (auto split: list.splits)
   subgoal
-    by (metis Nil_is_append_conv last_in_set last_snoc list.simps(3) set_takeWhileD)
-  subgoal
-    by (metis hd_dropWhile le_less_linear list.sel(1) list.simps(3))
+    apply (auto split: list.splits)
+    by (metis (no_types, lifting) case_prodD in_set_conv_decomp takeWhile_eq_all_conv takeWhile_idem)
+  subgoal by (metis case_prod_conv hd_dropWhile le_less_linear list.sel(1) list.simps(3))
+  subgoal using bplustree_linear_search_list.isin_list_set by blast
+  subgoal using bplustree_linear_search_list.insert_list_set by blast
+  subgoal using bplustree_linear_search_list.delete_list_set by blast
   done
 
 
 text "Some examples follow to show that the implementation works
       and the above lemmas make sense. The examples are visualized in the thesis."
 
-
-find_theorems bplustree_ls_isin_list
-
+abbreviation "bplustree\<^sub>q \<equiv> bplustree_ls_isin"
 abbreviation "bplustree\<^sub>i \<equiv> bplustree_ls_insert"
 abbreviation "bplustree\<^sub>d \<equiv> bplustree_ls_delete"
 
-typedef uint32 = "{n::nat. n \<le> 100}" 
+definition "uint8_max \<equiv> 2^8-1::nat"
+declare uint8_max_def[simp]
+
+typedef uint8 = "{n::nat. n \<le> uint8_max}" 
   by auto
 
-setup_lifting type_definition_uint32
+setup_lifting type_definition_uint8
 
-instantiation uint32 :: linorder
+instantiation uint8 :: linorder
 begin
 
-lift_definition less_eq_uint32 :: "uint32 \<Rightarrow> uint32 \<Rightarrow> bool"
+lift_definition less_eq_uint8 :: "uint8 \<Rightarrow> uint8 \<Rightarrow> bool"
   is "(less_eq::nat \<Rightarrow> nat \<Rightarrow> bool)" .
 
-lift_definition less_uint32 :: "uint32 \<Rightarrow> uint32 \<Rightarrow> bool"
+lift_definition less_uint8 :: "uint8 \<Rightarrow> uint8 \<Rightarrow> bool"
   is "(less::nat \<Rightarrow> nat \<Rightarrow> bool)" .
 
 instance
   by standard (transfer; auto)+
 end
 
-instantiation uint32 :: order_top
+instantiation uint8 :: order_top
 begin
 
-lift_definition top_uint32 :: uint32 is "100::nat"
+lift_definition top_uint8 :: uint8 is "uint8_max::nat"
   by simp
 
 
@@ -74,43 +87,52 @@ instance
 end
 
 
-instantiation uint32 :: numeral
+instantiation uint8 :: numeral
 begin
 
-lift_definition one_uint32 :: uint32 is "1::nat"
+lift_definition one_uint8 :: uint8 is "1::nat"
   by auto
 
-lift_definition plus_uint32 :: "uint32 \<Rightarrow> uint32 \<Rightarrow> uint32"
-  is "\<lambda>a b. min (a + b) (100)"
+lift_definition plus_uint8 :: "uint8 \<Rightarrow> uint8 \<Rightarrow> uint8"
+  is "\<lambda>a b. min (a + b) uint8_max"
   by simp
 
 instance by standard (transfer; auto)
 end
 
+instantiation uint8 :: equal
+begin
 
-(* the below will take ages to evaluate
+lift_definition equal_uint8 :: "uint8 \<Rightarrow> uint8 \<Rightarrow> bool"
+  is "(=)" .
 
-lemma [code]: "(2^32::nat) = 4294967296" 
-  by simp
+instance by standard (transfer; auto)
+end
 
-value "2^32::nat"
-*)
 
-value "let k=2::nat; x::uint32 bplustree = (Node [(Node [(LNode [1,2], 2),(LNode [3,4], 4),(LNode [5,6,7], 8)] (LNode [9,10]), 10)] (Node [(LNode [11,12,13,14], 14), (LNode [15,17], 20)] (LNode [21,22,23]))) in
+value "uint8_max"
+
+value "let k=2::nat; x::uint8 bplustree = (Node [(Node [(LNode [1,2], 2),(LNode [3,4], 4),(LNode [5,6,7], 8)] (LNode [9,10]), 10)] (Node [(LNode [11,12,13,14], 14), (LNode [15,17], 20)] (LNode [21,22,23]))) in
       root_order k x"
-value "let k=2::nat; x::uint32 bplustree = (Node [(Node [(LNode [1,2], 2),(LNode [3,4], 4),(LNode [5,6,7], 8)] (LNode [9,10]), 10)] (Node [(LNode [11,12,13,14], 14), (LNode [15,17], 20)] (LNode [21,22,23]))) in
+value "let k=2::nat; x::uint8 bplustree = (Node [(Node [(LNode [1,2], 2),(LNode [3,4], 4),(LNode [5,6,7], 8)] (LNode [9,10]), 10)] (Node [(LNode [11,12,13,14], 14), (LNode [15,17], 20)] (LNode [21,22,23]))) in
       bal x"
-value "let k=2::nat; x::uint32 bplustree = (Node [(Node [(LNode [1,2], 2),(LNode [3,4], 4),(LNode [5,6,7], 8)] (LNode [9,10]), 10)] (Node [(LNode [11,12,13,14], 14), (LNode [15,17], 20)] (LNode [50,55,56]))) in
-      sorted_less (inorder x)"
-value "let k=2::nat; x::uint32 bplustree = (Node [(Node [(LNode [1,2], 2),(LNode [3,4], 4),(LNode [5,6,7], 8)] (LNode [9,10]), 10)] (Node [(LNode [11,12,13,14], 14), (LNode [15,17], 20)] (LNode [50,55,56]))) in
+value "let k=2::nat; x::uint8 bplustree = (Node [(Node [(LNode [1,2], 2),(LNode [3,4], 4),(LNode [5,6,7], 8)] (LNode [9,10]), 10)] (Node [(LNode [11,12,13,14], 14), (LNode [15,17], 20)] (LNode [50,55,56]))) in
+      sorted_less (leaves x)"
+value "let k=2::nat; x::uint8 bplustree = (Node [(Node [(LNode [1,2], 2),(LNode [3,4], 4),(LNode [5,6,7], 8)] (LNode [9,10]), 10)] (Node [(LNode [11,12,13,14], 14), (LNode [15,17], 20)] (LNode [50,55,56]))) in
+      Laligned x top"
+value "let k=2::nat; x::uint8 bplustree = (Node [(Node [(LNode [1,2], 2),(LNode [3,4], 4),(LNode [5,6,7], 8)] (LNode [9,10]), 10)] (Node [(LNode [11,12,13,14], 14), (LNode [15,17], 20)] (LNode [50,55,56]))) in
       x"
-(*value "let k=2::nat; x::uint32 bplustree = (Node [(Node [(LNode [1,2], 2),(LNode [3,4], 4),(LNode [5,6,7], 8)] (LNode [9,10]), 10)] (Node [(LNode [11,12,13,14], 14), (LNode [15,17], 20)] (LNode [50,55,56]))) in
-      bplustree\<^sub>i k 9 x"*)
-value "let k=2::nat; x::uint32 bplustree = (Node [(Node [(Leaf, 3),(Leaf, 5),(Leaf, 6)] Leaf, 10)] (Node [(Leaf, 14), (Leaf, 20)] Leaf)) in
+value "let k=2::nat; x::uint8 bplustree = (Node [(Node [(LNode [1,2], 2),(LNode [3,4], 4),(LNode [5,6,7], 8)] (LNode [9,10]), 10)] (Node [(LNode [11,12,13,14], 14), (LNode [15,17], 20)] (LNode [50,55,56]))) in
+      bplustree\<^sub>q x 4"
+value "let k=2::nat; x::uint8 bplustree = (Node [(Node [(LNode [1,2], 2),(LNode [3,4], 4),(LNode [5,6,7], 8)] (LNode [9,10]), 10)] (Node [(LNode [11,12,13,14], 14), (LNode [15,17], 20)] (LNode [50,55,56]))) in
+      bplustree\<^sub>q x 20"
+value "let k=2::nat; x::uint8 bplustree = (Node [(Node [(LNode [1,2], 2),(LNode [3,4], 4),(LNode [5,6,7], 8)] (LNode [9,10]), 10)] (Node [(LNode [11,12,13,14], 14), (LNode [15,17], 20)] (LNode [50,55,56]))) in
+      bplustree\<^sub>i k 9 x"
+value "let k=2::nat; x::uint8 bplustree = (Node [(Node [(LNode [1,2], 2),(LNode [3,4], 4),(LNode [5,6,7], 8)] (LNode [9,10]), 10)] (Node [(LNode [11,12,13,14], 14), (LNode [15,17], 20)] (LNode [50,55,56]))) in
       bplustree\<^sub>i k 1 (bplustree\<^sub>i k 9 x)"
-value "let k=2::nat; x::uint32 bplustree = (Node [(Node [(Leaf, 3),(Leaf, 5),(Leaf, 6)] Leaf, 10)] (Node [(Leaf, 14), (Leaf, 20)] Leaf)) in
+value "let k=2::nat; x::uint8 bplustree = (Node [(Node [(LNode [1,2], 2),(LNode [3,4], 4),(LNode [5,6,7], 8)] (LNode [9,10]), 10)] (Node [(LNode [11,12,13,14], 14), (LNode [15,17], 20)] (LNode [50,55,56]))) in
       bplustree\<^sub>d k 10 (bplustree\<^sub>i k 1 (bplustree\<^sub>i k 9 x))"
-value "let k=2::nat; x::uint32 bplustree = (Node [(Node [(Leaf, 3),(Leaf, 5),(Leaf, 6)] Leaf, 10)] (Node [(Leaf, 14), (Leaf, 20)] Leaf)) in
+value "let k=2::nat; x::uint8 bplustree = (Node [(Node [(LNode [1,2], 2),(LNode [3,4], 4),(LNode [5,6,7], 8)] (LNode [9,10]), 10)] (Node [(LNode [11,12,13,14], 14), (LNode [15,17], 20)] (LNode [50,55,56]))) in
       bplustree\<^sub>d k 3 (bplustree\<^sub>d k 10 (bplustree\<^sub>i k 1 (bplustree\<^sub>i k 9 x)))"
 
 
